Upgrading Coq version

Eval.v
@@ -1,270 +1,247 @@
+From Coq Require Import Program.Basics.
+From Coq Require Import Strings.String.
+
 From Elo Require Import Core.
 
-Definition bind (o : option (mem * tm)) (f : tm -> tm)
-  : option (mem * tm) :=
-  match o with
-  | Some (m, t) => Some (m, (f t))
-  | None        => None
-  end.
-
-Local Notation "o '>>=' f" := (bind o f)
-  (no associativity, at level 10).
-
-Fixpoint eval (m : mem) (t : tm) : option (mem * tm) :=
-  let term2 := fun
-    (m : mem)
-    (t1 t2 : tm)
-    (cons : tm -> tm -> tm)
-    (result : option (mem * tm)) =>
-      if is_value t1 then
-        if is_value t2 then
-          result
-        else
-          eval m t2 >>= (fun t2' => cons t1 t2')
-      else
-        eval m t1 >>= (fun t1' => cons t1' t2)
-  in
-  match t with
-  | <{unit}> => Some (m, t)
-  (* --------------------------------------------------------------------- *)
-  | <{nat _}> => Some (m, t)
-  (* --------------------------------------------------------------------- *)
-  | <{t1 + t2}> => term2 m t1 t2 tm_plus (
-      match t with
-      | <{nat n1 + nat n2}> => Some (m, <{nat (n1 + n2)}>)
-      | _ => None
-      end)
-  (* --------------------------------------------------------------------- *)
-  | <{t1 - t2}> => term2 m t1 t2 tm_monus (
-      match t with
-      | <{nat n1 - nat n2}> => Some (m, <{nat (n1 - n2)}>)
-      | _ => None
-      end)
-  (* --------------------------------------------------------------------- *)
-  | <{t1; t2}> => if is_value t1
-                    then Some (m, t2)
-                    else eval m t1 >>= (fun t1' => <{t1'; t2}>)
-  (* --------------------------------------------------------------------- *)
-  | <{if t1 then t2 else t3 end}> => 
-    if is_value t1 then
-      match t1 with
-      | <{nat O    }> => Some (m, t3)
-      | <{nat (S _)}> => Some (m, t2)
-      | _ => None
-      end
-    else
-      eval m t1 >>= (fun t1' => <{if t1' then t2 else t3 end}>)
-  (* --------------------------------------------------------------------- *)
-  | <{while t1 do t2 end}> =>
-    let t' := <{if t1 then t2; while t1 do t2 end else unit end}> in
-    Some (m, t')
-  (* --------------------------------------------------------------------- *)
-  | <{var _}> => Some (m, t)
-  (* --------------------------------------------------------------------- *)
-  | <{fn _ _ _}> => Some (m, t)
-  (* --------------------------------------------------------------------- *)
-  | <{call t1 t2}> => term2 m t1 t2 tm_call (
-      match t with
-      | <{call (fn x _ t) tx}> => Some (m, <{[x := tx] t}>)
-      | _ => None
-      end)
-  (* --------------------------------------------------------------------- *)
-  | <{&_ : _}> => Some (m, t)
-  (* --------------------------------------------------------------------- *)
-  | <{new t : T}> => None
-  (* --------------------------------------------------------------------- *)
-  | <{init ad t : T}> => None
-  (* --------------------------------------------------------------------- *)
-  | <{*t}> => None
-  (* --------------------------------------------------------------------- *)
-  | <{t1 := t2}> => None
-  (* --------------------------------------------------------------------- *)
-  | <{acq t1 x t2}> => None
-  (* --------------------------------------------------------------------- *)
-  | <{cr ad t}> => None
-  (* --------------------------------------------------------------------- *)
-  | <{spawn t}> => None
-  end.
-
-
-
-
-
-
-
-
-
-
-
-
-
-
-
-
-
-
-
-
-
-
-
-
-
-
-
-
-
-
-
-
-
-
-
-
-
-
-
-
-
-
-
-
-
-
-
-Inductive state : Set :=
-  | done    : mem  -> tm -> state
-  | waiting : addr -> tm -> state
-  | error   : state
-  | oog     : state
+Inductive Result : Set :=
+  | Ok      : mem -> tm -> Result
+  | Spawn   : mem -> tm -> tm -> Result
+  | Waiting : addr -> Result
+  | Error   : string -> Result
   .
 
-Definition ret (m : mem) (o : option tm) : state :=
-  match o with
-  | Some t => done m t
-  | None   => error
+Definition bind (r : Result) (f : tm -> tm) : Result :=
+  match r with
+  | Ok m t       => Ok m (f t)
+  | Spawn m t t' => Spawn m (f t) t'
+  | Waiting ad   => Waiting ad
+  | Error s      => Error s
   end.
 
-Definition bind (s : state) (f : mem -> tm -> state) : state :=
-  match s with
-  | done m t => f m t
-  | _        => s
-  end.
+Local Notation "r '>>=' f" := (bind r f) (no associativity, at level 10).
 
-Local Notation "m ',' t '<-' s1 ';;' s2" := (bind s1 (fun m t => s2))
-  (right associativity, at level 84, t at next level, s1 at next level).
-
-Local Notation "s1 ';;' s2" := (bind s1 (fun _ _ => s2))
-  (at level 100, right associativity).
-
-Definition eplus (t1 t2 : tm) : option tm :=
-  match t1 with
-  | <{nat n1}> => match t2 with
-                  | <{nat n2}> => Some <{nat (n1 + n2)}>
-                  | _          => None
-                  end
-  | _ => None
-  end.
-
-Definition emonus (t1 t2 : tm) : option tm :=
-  match t1 with
-  | <{nat n1}> => match t2 with
-                  | <{nat n2}> => Some <{nat (n1 - n2)}>
-                  | _          => None
-                  end
-  | _ => None
-  end.
-
-Definition eif (t1 t2 t3 : tm) : option tm :=
-  match t1 with
-  | <{nat O    }> => Some t3
-  | <{nat (S _)}> => Some t2
-  | _             => None
-  end.
-
-Definition ecall (t tx : tm) : option tm :=
+Definition _plus m t : Result :=
   match t with
-  | <{fn x _ t'}> => Some <{[x := tx]t'}>
-  | _ => None
+  | <{nat n1 + nat n2}> => Ok m <{nat (n1 + n2)}>
+  | _ => Error "expecting <{_ + _}>"
   end.
 
-Definition eload (m : mem) (t : tm) : option tm :=
+Definition _monus m t : Result :=
   match t with
-  | <{&ad : _}> => m[ad].t
-  | _           => None
+  | <{nat n1 - nat n2}> => Ok m <{nat (n1 - n2)}>
+  | _ => Error "expecting <{_ - _}>"
   end.
 
-Definition easg (m : mem) (t1 t2 : tm) : state :=
-  match t1 with
-  | <{&ad : T}> => ret m[ad.t <- t2] (Some <{unit}>)
-  | _ => error
+Definition C_if t2 t3 := fun t1' => <{if t1' then t2 else t3 end}>.
+
+Definition _if m t : Result :=
+  match t with
+  | <{if nat O     then t2 else t3 end}> => Ok m t3
+  | <{if nat (S _) then t2 else t3 end}> => Ok m t2
+  | _ => Error "expecting <{if _ then _ else _ end}>"
   end.
 
-Definition eacq (m : mem) (t1 : tm) (x : id) (t2 : tm) : state :=
-  match t1 with
-  | <{&ad : T}> => 
+Definition _while (m : mem) t1 t2 :=
+  Ok m <{if t1 then t2; while t1 do t2 end else unit end}>.
+
+Definition _call m t : Result :=
+  match t with
+  | <{call (fn x _ t) tx}> => Ok m <{[x := tx] t}>
+  | _ => Error "expecting <{call (fn _ _ _) _}>"
+  end.
+
+Definition _new m t T :=
+  let ad := #m in Ok (m +++ new_cell T) <{init ad t : T}>.
+
+Definition C_init ad T := fun t' => <{init ad t' : T}>.
+
+Definition _init m t : Result :=
+  match t with
+  | <{init ad t : T}> => Ok m[ad.t <- t] <{&ad : T}>
+  | _ => Error "expecting <{init _ _ : _}>"
+  end.
+
+Definition _load m t : Result :=
+  match t with
+  | <{* (&ad : T)}> =>
     match m[ad].t with
-    | Some tx =>
-      if m[ad].X
-        then waiting ad <{acq t1 x t2}>
-        else ret m[ad.X <- true] (Some <{[x := tx]t2}>)
-    | None => error
-    end
-  | _ => error
+    | Some t => Ok m t
+    | None   => Error "attempt to read empty memory cell"
+    end  
+  | _ => Error "expecting <{* (&_ : _)}>"
   end.
 
-Fixpoint eval (m : mem) (t : tm) (i : nat) : state :=
-  match i with
-  | O    => oog
-  | S i' =>
-    match t with
-    | <{unit }> => done m t
-    | <{nat n}> => done m t
-    (* --- *)
-    | <{t1 + t2}> =>
-      m',  t1' <- eval m  t1 i' ;;
-      m'', t2' <- eval m' t2 i' ;;
-      ret m'' (eplus t1' t2')
-    | <{t1 - t2}> =>
-      m',  t1' <- eval m  t1 i' ;;
-      m'', t2' <- eval m' t2 i' ;;
-      ret m'' (emonus t1' t2')
-    | <{t1; t2}> =>
-      m',  t1' <- eval m  t1 i' ;;
-      m'', t2' <- eval m' t2 i' ;;
-      ret m'' (Some t2')
-    | <{if t1 then t2 else t3 end}> =>
-      m',  t1' <- eval m  t1 i' ;;
-      ret m' (eif t1' t2 t3)
-    | <{while t1 do t2 end}> =>
-      eval m <{if t1 then t2; while t1 do t2 end else unit end}> i'
-    (* --- *)
-    | <{var _     }> => error
-    | <{fn _ _ _  }> => error
-    | <{call t1 t2}> =>
-      m',  t1' <- eval m  t1 i' ;;
-      m'', t2' <- eval m' t2 i' ;;
-      ret m'' (ecall t1' t2')
-    (* --- *)
-    | <{&_ : _   }> => error
-    | <{new t : T}> =>
-      let ad := #m in
-      ret (m +++ (_cell None T false R_invalid)) (Some <{init ad t : T}>)
-    | <{init ad t : T}> =>
-      m', t' <- eval m t i' ;;
-      ret m'[ad.t <- t'] (Some <{&ad : T}>)
-    | <{*t}> =>
-      m', t' <- eval m t i' ;;
-      ret m' (eload m' t')
-    | <{t1 := t2}> =>
-      m',  t1' <- eval m  t1 i' ;;
-      m'', t2' <- eval m' t2 i' ;;
-      easg m'' t1' t2'
-    | <{acq t1 x t2}> =>
-      m', t1' <- eval m t1 i' ;;
-      eacq m' t1' x t2
-    (* --- *)
-    | _ => error
-    end
+Definition _asg m t : Result :=
+  match t with
+  | <{(&ad : T) := t}> => Ok m[ad.t <- t] <{unit}>
+  | _ => Error "expecting <{(&_ : _) := _}>"
   end.
+
+Definition C_acq x t2 := fun t1' => <{acq t1' x t2}>.
+
+Definition _acq m t : Result :=
+  match t with
+  | <{acq (&ad : T) x t}> =>
+    if m[ad].X then
+      Waiting ad
+    else
+      match m[ad].t with
+      | Some tx => Ok m[ad.X <- true] <{cr ad ([x := tx]t)}>
+      | None    => Error "attempt to read empty memory cell"
+      end
+  | _ => Error "expecting <{acq (&_ : _) _ _}>"
+  end.
+
+Definition _cr m t : Result :=
+  match t with
+  | <{cr ad t}> => Ok m[ad.X <- false] t
+  | _ => Error "expecting <{cr _ _}>"
+  end.
+
+Fixpoint eval (m : mem) (t : tm) : Result :=
+  let do1 := fun m t (C : tm -> tm) (R : Result) =>
+    if is_value t then R else eval m t >>= C
+  in
+  let do2 := fun m t1 t2 (C : tm -> tm -> tm) (R : Result) =>
+    do1 m t1 (flip C t2) (do1 m t2 (C t1) R)
+  in
+  match t with
+  | <{unit                     }> => Ok m t
+  | <{nat _                    }> => Ok m t
+  | <{t1 + t2                  }> => do2 m t1 t2 tm_plus (_plus m t)
+  | <{t1 - t2                  }> => do2 m t1 t2 tm_monus (_monus m t)
+  | <{t1; t2                   }> => do1 m t1 (flip tm_seq t2) (Ok m t2)
+  | <{if t1 then t2 else t3 end}> => do1 m t1 (C_if t2 t3) (_if m t)
+  | <{while t1 do t2 end       }> => _while m t1 t2
+  | <{var _                    }> => Ok m t
+  | <{fn _ _ _                 }> => Ok m t
+  | <{call t1 t2               }> => do2 m t1 t2 tm_call (_call m t)
+  | <{&_ : _                   }> => Ok m t
+  | <{new t : T                }> => _new m t T
+  | <{init ad t' : T           }> => do1 m t' (C_init ad T) (_init m t)
+  | <{*t'                      }> => do1 m t' tm_load (_load m t)
+  | <{t1 := t2                 }> => do2 m t1 t2 tm_asg (_asg m t)
+  | <{acq t1 x t2              }> => do1 m t1 (C_acq x t2) (_acq m t)
+  | <{cr ad t'                 }> => do1 m t' (tm_cr ad) (_cr m t)
+  | <{spawn t'                 }> => Spawn m <{unit}> t'
+  end.
+
+(* -------------------------------------------------------------------------- *)
+
+Local Lemma isvalue_from_tstep : forall t1 t2 e,
+  t1 --[e]--> t2 ->
+  is_value t1 = false.
+Proof.
+  intros. destruct t1; invc_tstep; cbv; reflexivity.
+Qed.
+
+Local Lemma isvalue_from_value : forall t,
+  value t ->
+  is_value t = true.
+Proof.
+  intros * Hval. destruct t; invc Hval; cbv; reflexivity.
+Qed.
+
+Local Lemma isvalue_from_notvalue : forall t,
+  ~ value t ->
+  is_value t = false.
+Proof.
+  intros * Hval. destruct t; auto; exfalso; eauto using value.
+Qed.
+
+Local Ltac iota :=
+  match goal with
+  | Htstep : ?t --[?e]--> ?t'
+  |- context[if is_value ?t then _ else _] =>
+    rewrite (isvalue_from_tstep t t' e Htstep)
+  (* --- *)
+  | Htstep : ?t --[?e]--> ?t'
+  , Hif : context[if is_value ?t then _ else _]
+  |- _ =>
+    rewrite (isvalue_from_tstep t t' e Htstep) in Hif
+  (* --- *)
+  | Hval : value ?t
+  |- context[if is_value ?t then _ else _] =>
+    rewrite (isvalue_from_value t Hval)
+  (* --- *)
+  | Hval : value ?t
+  , Hif : context[if is_value ?t then _ else _]
+  |- _ =>
+    rewrite (isvalue_from_value t Hval) in Hif
+  (* --- *)
+  | Hnval : ~ value ?t
+  |- context[if is_value ?t then _ else _] =>
+    rewrite (isvalue_from_notvalue t Hnval)
+  (* --- *)
+  | Hnval : ~ value ?t
+  , Hif : context[if is_value ?t then _ else _]
+  |- _ =>
+    rewrite (isvalue_from_notvalue t Hnval) in Hif
+  (* --- *)
+  | |- context[if is_value <{&?ad : ?T}> then _ else _] =>
+    rewrite (isvalue_from_value <{&ad : T}>); eauto using value
+  | Hif : context[if is_value <{&?ad : ?T}> then _ else _] |- _ =>
+    rewrite (isvalue_from_value <{&ad : T}>) in Hif; eauto using value
+  end.
+
+(* -------------------------------------------------------------------------- *)
+
+Local Lemma mstep_to_eval : forall m1 m2 t1 t2 e,
+  m1 \ t1 ==[e]==> m2 \ t2 ->
+  eval m1 t1 = Ok m2 t2.
+Proof.
+  intros. invc_mstep;
+  ind_tstep; repeat spec;
+  unfold eval; fold eval; repeat iota; trivial;
+  try rewrite IHtstep; unfold flip; simpl; trivial.
+  - destruct (m2[ad].t); auto. invc_eq. reflexivity.
+  - destruct (m1[ad].X); auto. destruct (m1[ad].t); auto. invc_eq. trivial.
+Qed.
+
+(* -------------------------------------------------------------------------- *)
+
+Local Lemma eval_value : forall m t,
+  value t ->
+  eval m t = Ok m t.
+Proof.
+  intros * Hval. invc Hval; trivial.
+Qed.
+
+Local Lemma eval_to_mstep : forall m1 m2 t1 t2,
+  eval m1 t1 = Ok m2 t2 ->
+  value t1 \/ exists e, m1 \ t1 ==[e]==> m2 \ t2.
+Proof.
+  intros * Heq. gendep t2. gendep m2.
+  induction t1; intros;
+  try solve [left; auto using value];
+  right.
+  - unfold eval in Heq. fold eval in Heq.
+    destruct (value_dec t1_1), (value_dec t1_2); repeat iota.
+    + destruct t1_1; try solve [invc Heq].
+      destruct t1_2; invc Heq.
+      eauto using tstep, mstep.
+    + specialize (IHt1_1 m1 t1_1).
+      rewrite eval_value in IHt1_1; trivial.
+      specialize (IHt1_1 eq_refl) as [? | [? ?]].
+      * clean.
+        unfold bind in Heq.
+        destruct (eval m1 t1_2); invc Heq.
+        specialize (IHt1_2 m2 t eq_refl) as [? | [? ?]]; auto.
+        exists x. invc_mstep; eauto using tstep, mstep.
+      * invc_mstep; value_does_not_step.
+    + specialize (IHt1_2 m1 t1_2).
+      rewrite eval_value in IHt1_2; trivial.
+      specialize (IHt1_2 eq_refl) as [? | [? ?]].
+      * clean.
+        unfold bind in Heq.
+        destruct (eval m1 t1_1); invc Heq.
+        specialize (IHt1_1 m2 t eq_refl) as [? | [? ?]]; auto.
+        exists x. invc_mstep; eauto using tstep, mstep.
+      * invc_mstep; value_does_not_step.
+    + unfold bind in Heq.
+      destruct (eval m1 t1_1); invc Heq.
+      specialize (IHt1_1 m2 t eq_refl) as [? | [? ?]]; auto.
+      exists x. invc_mstep; eauto using tstep, mstep.
+  - admit.
+Qed.
 
