Values.v
@@ -27,7 +27,7 @@ Qed.
 
 Theorem value_preservation_cstep : forall m1 m2 ths1 ths2 tid e,
   forall_memory m1 value ->
-  m1 / ths1 ~~[tid, e]~~> m2 / ths2 ->
+  m1 \ ths1 ~~[tid, e]~~> m2 \ ths2 ->
   forall_memory m2 value.
 Proof.
   intros. invc_cstep; trivial. invc_mstep; trivial;
@@ -36,19 +36,19 @@ Qed.
 
 Theorem value_preservation_rstep : forall m1 m2 ths1 ths2 tid e,
   forall_memory m1 value ->
-  m1 / ths1 ~~~[tid, e]~~> m2 / ths2 ->
+  m1 \ ths1 ~~~[tid, e]~~> m2 \ ths2 ->
   forall_memory m2 value.
 Proof.
   intros. invc_rstep; eauto using value_preservation_cstep.
-  match goal with _ : _ / _ ~~[_, _]~~> ?m / ?ths |- _ =>
+  match goal with _ : _ \ _ ~~[_, _]~~> ?m \ ?ths |- _ =>
     assert (forall_memory m value) by eauto using value_preservation_cstep
   end.
-  repeat intro; repeat omicron; upsilon; eauto.
+  repeat intro; repeat omicron; upsilon; auto; eauto.
 Qed.
 
 Theorem value_preservation_ustep : forall m1 m2 ths1 ths2 tc,
   forall_memory m1 value ->
-  m1 / ths1 ~~[tc]~~>* m2 / ths2 ->
+  m1 \ ths1 ~~[tc]~~>* m2 \ ths2 ->
   forall_memory m2 value.
 Proof.
   intros. ind_ustep; eauto using value_preservation_rstep.
